theories/L6_PCPS/shrink_cps_corresp.v
@@ -4,6 +4,8 @@ Require Import Coq.Setoids.Setoid.
 Require Import Coq.Classes.Morphisms.
 Import RelationClasses.
 
+
+
 Require Import ExtLib.Data.Bool.
 Require Libraries.Maps.
 Require Coq.funind.Recdef.
@@ -15,7 +17,7 @@ Require Import Libraries.maps_util.
 Require Import Libraries.Coqlib L6.Ensembles_util. 
 Require Import L6.cps.
 Require Import L6.ctx L6.logical_relations.
-Require Import L6.cps_util L6.List_util L6.shrink_cps L6.eval L6.set_util L6.identifiers  L6.set_util.
+Require Import L6.cps_util L6.List_util L6.shrink_cps L6.eval L6.set_util L6.identifiers  L6.stemctx.
 Require Import L6.shrink_cps_correct.
 
 
@@ -897,295 +899,15 @@ Section CONTRACT.
   Qed.
 
 
-  Fixpoint name_in_fundefs_ctx B:=
-    match B with
-      | Fcons1_c f' _ _ _ B0 => Union var [set f'] (name_in_fundefs B0)
-      | Fcons2_c f' _ _ _ B0 => Union var [set f'] (name_in_fundefs_ctx B0)
-    end.
+
+
   
 
 
-  (** bound_stem_ctx represents the bound variables on the stem (from the root to the hole) *)
-  Inductive bound_stem_ctx: exp_ctx -> Ensemble var  :=
-  | Bound_Constr1_c: forall v t ys c,
-                       bound_stem_ctx (Econstr_c v t ys c) v
-  | Bound_Constr2_c: forall c v v' t ys,
-                       bound_stem_ctx c v ->
-                       bound_stem_ctx (Econstr_c v' t ys c) v
-  | Bound_Proj1_c: forall  t n r c v,
-                     bound_stem_ctx (Eproj_c v t n r c) v
-  | Bound_Proj2_c: forall  t n r c v' v,
-                     bound_stem_ctx c v' ->
-                     bound_stem_ctx (Eproj_c v t n r c) v'
-  | Bound_Prim1_c: forall  x f ys c,
-                     bound_stem_ctx (Eprim_c x f ys c) x
-  | Bound_Prim2_c: forall  t r c v' v,
-                     bound_stem_ctx c v' ->
-                     bound_stem_ctx (Eprim_c v t r c) v'
-  | Bound_Case1_c: forall v v' lce t c lce',
-                     bound_stem_ctx c v' ->
-                     bound_stem_ctx (Ecase_c v lce t c lce') v'
-  | Bound_Fun11_c: forall fds v c,
-                     name_in_fundefs fds v ->
-                     bound_stem_ctx (Efun1_c fds c) v
-  | Bound_Fun12_c: forall fds v c,
-                     bound_stem_ctx c v ->
-                     bound_stem_ctx (Efun1_c fds c) v
-  | Bound_Fun21_c: forall fds v c,
-                     name_in_fundefs_ctx fds v ->
-                     bound_stem_ctx (Efun2_c fds c) v 
-
-  | Bound_Fun2_c: forall cfds v e,
-                    bound_stem_fundefs_ctx cfds v ->
-                    bound_stem_ctx (Efun2_c cfds e) v
-  with bound_stem_fundefs_ctx: fundefs_ctx -> Ensemble var :=
-                                                  | Bound_Fcons11_c: forall f t xs c fds v,
-                                                                       List.In v xs ->
-                                                                       bound_stem_fundefs_ctx (Fcons1_c f t xs c fds) v
-
-                                                  | Bound_Fcons12_c: forall f t xs c fds v,
-                                                                       bound_stem_ctx c v ->
-                                                                       bound_stem_fundefs_ctx (Fcons1_c f t xs c fds) v
-                                                  | Bound_Fcons2_c: forall f t xs e cfds v,
-                                                                      bound_stem_fundefs_ctx cfds v ->
-                                                                      bound_stem_fundefs_ctx (Fcons2_c f t xs e cfds) v.
-
-  Hint Constructors bound_stem_ctx.
-  Hint Constructors bound_stem_fundefs_ctx.
-
-
-  Lemma bound_stem_Econstr_c x t ys c :
-    Same_set _ (bound_stem_ctx (Econstr_c x t ys c))
-             (Union var (bound_stem_ctx c) (Singleton _ x)).
-  Proof.
-    split; intros x' H; inv H; eauto. inv H0; eauto.
-  Qed.
-
-  Lemma bound_stem_Eproj_c v t n r c :
-    Same_set _ (bound_stem_ctx (Eproj_c v t n r c))
-             (Union var (bound_stem_ctx c) (Singleton _ v)).
-  Proof.
-    split; intros x' H; inv H; eauto. inv H0; eauto.
-  Qed.
-
-  Lemma bound_stem_Eprim_c x tau y c :
-    Same_set _ (bound_stem_ctx (Eprim_c x tau y c))
-             (Union var (bound_stem_ctx c) (Singleton _ x)).
-  Proof.
-    split; intros x' H; inv H; eauto. inv H0; eauto.
-  Qed.
-
-  Lemma bound_stem_Hole_c :
-    Same_set _ (bound_stem_ctx Hole_c)
-             (Empty_set var).
-  Proof.
-    split; intros x' H; inv H; eauto. 
-  Qed.
-
-  Lemma bound_stem_Case_c :
-    forall v  lce t c lce',
-      Same_set _ (bound_stem_ctx (Ecase_c v lce t c lce'))
-               (bound_stem_ctx c).
-  Proof with eauto with Ensembles_DB.
-    split; intros; intro; intros.
-    - inversion H; subst; eauto.
-    - constructor.
-      auto.
-  Qed.
-
-
-  Lemma bound_stem_Fun1_c :
-    forall fds c,
-      Same_set _ (bound_stem_ctx (Efun1_c fds c))
-               (Union _ (name_in_fundefs fds) (bound_stem_ctx c)).
-  Proof.
-    split; intros x H; inv H; eauto.
-  Qed.
-
-  Lemma bound_stem_Fun2_c :
-    forall cfds e,
-      Same_set _ (bound_stem_ctx (Efun2_c cfds e))
-               (Union _ (name_in_fundefs_ctx cfds) (bound_stem_fundefs_ctx cfds)).
-  Proof.
-    split; intros x H; inv H; eauto.
-  Qed.
-
-  Lemma bound_stem_Fcons1_c :
-    forall c v l e0 f,
-      Same_set _ (bound_stem_fundefs_ctx (Fcons1_c v c l e0 f))
-               (Union _ (bound_stem_ctx e0) (FromList l)).             
-  Proof.
-    split; intros x H; inv H; eauto.
-  Qed.  
-
-  Lemma bound_stem_Fcons2_c :
-    forall c v l e0 f,
-      Same_set _ (bound_stem_fundefs_ctx (Fcons2_c v c l e0 f))
-               (bound_stem_fundefs_ctx f).             
-  Proof.
-    split; intros x H; inv H; eauto.
-  Qed.
 
 
 
 
-  Ltac normalize_bound_stem_ctx' :=
-    match goal with
-      | [ |- context[bound_stem_ctx Hole_c]] =>
-        rewrite bound_stem_Hole_c 
-      | [|- context[bound_stem_ctx (Econstr_c _ _ _ _)]] =>
-        rewrite bound_stem_Econstr_c
-      | [|- context[bound_stem_ctx (Eproj_c _ _ _ _ _)]] =>
-        rewrite bound_stem_Eproj_c
-      | [|- context[bound_stem_ctx (Ecase_c _ _ _ _ _)]] =>
-        rewrite bound_stem_Case_c
-      | [ |- context[bound_stem_ctx (Efun1_c _ _)]] =>
-        rewrite bound_stem_Fun1_c 
-      | [ |- context[bound_stem_ctx (Efun2_c _ _)] ] =>
-        rewrite bound_stem_Fun2_c
-      | [|- context[bound_stem_ctx (Eprim_c _ _ _ _)]] =>
-        rewrite bound_stem_Eprim_c
-      | [|- context[bound_stem_fundefs_ctx (Fcons1_c _ _ _ _ _)]] =>
-        rewrite bound_stem_Fcons1_c
-      | [|- context[bound_stem_fundefs_ctx (Fcons2_c _ _ _ _ _)]] =>
-        rewrite bound_stem_Fcons2_c
-    end.
-
-  Ltac normalize_bound_stem_ctx_in_ctx' :=
-    match goal with
-      | [ H: context[bound_stem_ctx Hole_c] |- _] =>
-        rewrite bound_stem_Hole_c in H
-      | [ H : context[bound_stem_ctx (Econstr_c _ _ _ _)] |- _ ] =>
-        rewrite bound_stem_Econstr_c in H
-      | [ H : context[bound_stem_ctx (Eproj_c _ _ _ _ _)]  |- _ ] =>
-        rewrite bound_stem_Eproj_c in H
-      | [H: context[bound_stem_ctx (Ecase_c _ _ _ _ _)] |- _] =>
-        rewrite bound_stem_Case_c in H
-      | [ H : context[bound_stem_ctx (Efun1_c _ _)] |- _ ] =>
-        rewrite bound_stem_Fun1_c in H
-      | [ H : context[bound_stem_ctx (Efun2_c _ _)] |- _ ] =>
-        rewrite bound_stem_Fun2_c in H
-      | [ H : context[bound_stem_ctx (Eprim_c _ _ _ _)] |- _ ] =>
-        rewrite bound_stem_Eprim_c in H
-      | [H:context[bound_stem_fundefs_ctx (Fcons1_c _ _ _ _ _)] |- _] =>
-        rewrite bound_stem_Fcons1_c in H
-      | [H: context[bound_stem_fundefs_ctx (Fcons2_c _ _ _ _ _)] |- _] =>
-        rewrite bound_stem_Fcons2_c in H
-    end.
-
-
-  Ltac normalize_bound_var_ctx' :=
-    match goal with
-      | [ |- context[bound_var_ctx Hole_c]] =>
-        rewrite bound_var_Hole_c 
-      | [|- context[bound_var_ctx (Econstr_c _ _ _ _)]] =>
-        rewrite bound_var_Econstr_c
-      | [|- context[bound_var_ctx (Eproj_c _ _ _ _ _)]] =>
-        rewrite bound_var_Eproj_c
-      | [|- context[bound_var_ctx (Ecase_c _ _ _ _ _)]] =>
-        rewrite bound_var_Case_c
-      | [ |- context[bound_var_ctx (Efun1_c _ _)]] =>
-        rewrite bound_var_Fun1_c 
-      | [ |- context[bound_var_ctx (Efun2_c _ _)] ] =>
-        rewrite bound_var_Fun2_c
-      | [|- context[bound_var_ctx (Eprim_c _ _ _ _)]] =>
-        rewrite bound_var_Eprim_c
-      | [|- context[bound_var_fundefs_ctx (Fcons1_c _ _ _ _ _)]] =>
-        rewrite bound_var_Fcons1_c
-      | [|- context[bound_var_fundefs_ctx (Fcons2_c _ _ _ _ _)]] =>
-        rewrite bound_var_Fcons2_c
-    end.
-
-  Ltac normalize_bound_var_ctx_in_ctx' :=
-    match goal with
-      | [ H: context[bound_var_ctx Hole_c] |- _] =>
-        rewrite bound_var_Hole_c in H
-      | [ H : context[bound_var_ctx (Econstr_c _ _ _ _)] |- _ ] =>
-        rewrite bound_var_Econstr_c in H
-      | [ H : context[bound_var_ctx (Eproj_c _ _ _ _ _)]  |- _ ] =>
-        rewrite bound_var_Eproj_c in H
-      | [H: context[bound_var_ctx (Ecase_c _ _ _ _ _)] |- _] =>
-        rewrite bound_var_Case_c in H
-      | [ H : context[bound_var_ctx (Efun1_c _ _)] |- _ ] =>
-        rewrite bound_var_Fun1_c in H
-      | [ H : context[bound_var_ctx (Efun2_c _ _)] |- _ ] =>
-        rewrite bound_var_Fun2_c in H
-      | [ H : context[bound_var_ctx (Eprim_c _ _ _ _)] |- _ ] =>
-        rewrite bound_var_Eprim_c in H
-      | [H:context[bound_var_fundefs_ctx (Fcons1_c _ _ _ _ _)] |- _] =>
-        rewrite bound_var_Fcons1_c in H
-      | [H: context[bound_var_fundefs_ctx (Fcons2_c _ _ _ _ _)] |- _] =>
-        rewrite bound_var_Fcons2_c in H
-    end.
-
-
-
-
-  Theorem name_in_fundefs_ctx_bound_var_fundefs :
-    forall B, name_in_fundefs_ctx B \subset bound_var_fundefs_ctx B.
-  Proof.
-    intros.
-    induction B; normalize_bound_var_ctx'; simpl; eauto with Ensembles_DB.
-    assert (Hf4 := name_in_fundefs_bound_var_fundefs f).
-    eauto with Ensembles_DB.
-  Qed.
-
-  Theorem bound_stem_var:
-    (forall c,
-       Included _ (bound_stem_ctx c) (bound_var_ctx c))
-    /\
-    (forall fc, Included _ (bound_stem_fundefs_ctx fc) (bound_var_fundefs_ctx fc)).
-  Proof.
-    apply exp_fundefs_ctx_mutual_ind; intros; normalize_bound_var_ctx'; normalize_bound_stem_ctx'; eauto with Ensembles_DB.
-    assert (Hf4 := name_in_fundefs_bound_var_fundefs f4).
-    eauto with Ensembles_DB.
-
-    assert (Hf5 := name_in_fundefs_ctx_bound_var_fundefs f5).
-    eauto with Ensembles_DB.
-  Qed.
-
-  Theorem name_in_fundefs_ctx_comp:
-    forall c,
-    forall f5,
-      (name_in_fundefs_ctx (comp_f_ctx_f f5 c) <-->
-                           (name_in_fundefs_ctx f5)).
-  Proof.
-    intro c.
-    induction f5; simpl; eauto with Ensembles_DB.
-  Qed.
-
-  (** The set of bound variables of a composed context is equal to the union of the sets of bound variables of its constituents *)
-  Theorem bound_stem_comp_ctx_mut:
-    forall c',
-      (forall c,
-         Same_set _ (Union _ (bound_stem_ctx c) (bound_stem_ctx c')) (bound_stem_ctx (comp_ctx_f c c'))) /\
-      (forall fc,
-         Same_set  _ (Union _ (bound_stem_fundefs_ctx fc) (bound_stem_ctx c')) (bound_stem_fundefs_ctx (comp_f_ctx_f fc c'))).
-  Proof.
-    intro c'; apply exp_fundefs_ctx_mutual_ind; intros; simpl; repeat normalize_bound_stem_ctx'; eauto 25 with Ensembles_DB.
-    -  rewrite <- H.
-       rewrite <- Union_assoc.
-       rewrite Union_commut with (s1 := [set v]).
-       eauto 25 with Ensembles_DB.
-    - rewrite <- H.
-      rewrite <- Union_assoc.
-      rewrite Union_commut with (s1 := [set v]).
-      eauto 25 with Ensembles_DB.
-    -  rewrite <- H.
-       rewrite <- Union_assoc.
-       rewrite Union_commut with (s1 := [set v]).
-       eauto 25 with Ensembles_DB. 
-    -   rewrite <- H.
-        rewrite <- Union_assoc.
-        reflexivity.
-    - assert (Hf5 := name_in_fundefs_ctx_comp c' f5).
-      rewrite Hf5.
-      rewrite <- H.
-      eauto 25 with Ensembles_DB.
-    - rewrite <- H.
-      split;
-        eauto 25 with Ensembles_DB.
-  Qed.
 
   Theorem num_occur_case_le :
     forall x v e m cl,
@@ -2317,17 +2039,7 @@ Section CONTRACT.
     split; auto.
   Qed.
 
-  Print name_in_fundefs.
-  (* Section move_to_identifiers. *)
-  Theorem name_in_fundefs_ctx_ctx:
-    forall e cf, 
-      Same_set _ (name_in_fundefs_ctx cf) (name_in_fundefs (cf <[ e ]>)).
-  Proof.
-    induction cf.
-    simpl. eauto with Ensembles_DB.
-    simpl. rewrite IHcf.
-    eauto with Ensembles_DB.
-  Qed.         
+
 
   (** set of free variables for an applicative context *)
   Inductive occurs_free_ctx : exp_ctx -> Ensemble var :=
@@ -2370,7 +2082,7 @@ Section CONTRACT.
         occurs_free_ctx (Efun1_c defs e) y
   | Free_Efun21 :
       forall y defs e,
-        ~ (name_in_fundefs_ctx defs y) -> 
+        ~ (names_in_fundefs_ctx defs y) -> 
         occurs_free e y ->
         occurs_free_ctx (Efun2_c defs e) y                             
   | Free_Efun12 :
@@ -2407,7 +2119,7 @@ Section CONTRACT.
             forall x f tau ys e defs,  
               x <> f ->
               ~ (List.In x ys) ->
-              ~ (name_in_fundefs_ctx defs x) ->
+              ~ (names_in_fundefs_ctx defs x) ->
               occurs_free e x ->
               occurs_free_fundefs_ctx (Fcons2_c f tau ys e defs) x
         | Free_Fcons22 :
@@ -2460,7 +2172,7 @@ Section CONTRACT.
   Lemma occurs_free_Efun2_c B e :
     Same_set var (occurs_free_ctx (Efun2_c B e))
              (Union _ (occurs_free_fundefs_ctx B)
-                    (Setminus _ (occurs_free e) (name_in_fundefs_ctx B))).
+                    (Setminus _ (occurs_free e) (names_in_fundefs_ctx B))).
   Proof.
     split; intros x' H; inv H; eauto.
     right; eauto. constructor; eauto.
@@ -2502,7 +2214,7 @@ Section CONTRACT.
              (Union var (Setminus var (occurs_free e)
                                   (Union var (Singleton var f)
                                          (Union var (FromList xs)
-                                                (name_in_fundefs_ctx B))))
+                                                (names_in_fundefs_ctx B))))
                     (Setminus var (occurs_free_fundefs_ctx B) (Singleton var f))).
   Proof.
     split; intros x H; inv H.
@@ -2609,36 +2321,6 @@ Section CONTRACT.
     end.
 
 
-  Theorem bound_var_ctx_comp_ctx:      
-    (forall c1 c2,
-       Same_set _ (bound_var_ctx (comp_ctx_f c1 c2))
-                (Union _ (bound_var_ctx c1) (bound_var_ctx c2)))/\
-    (forall fc1 c2,
-       Same_set _ (bound_var_fundefs_ctx (comp_f_ctx_f fc1 c2))
-                (Union _ (bound_var_fundefs_ctx fc1) (bound_var_ctx c2)))
-  .
-  Proof.
-    exp_fundefs_ctx_induction IHc1 IHfc1; simpl; split; repeat (normalize_bound_var_ctx'); try (rewrite IHc1); try (rewrite IHfc1); repeat (normalize_bound_var_ctx'); repeat (normalize_bound_var); eauto 25 with Ensembles_DB.
-  Qed.
-
-  Ltac  normalize_bound_var_ctx :=
-    first [
-        match goal with
-          | [|- context[bound_var_ctx (comp_ctx_f _ _)]] =>
-            rewrite (proj1 (bound_var_ctx_comp_ctx))
-          | [|- context [bound_var_fundefs_ctx (comp_f_ctx_f _ _)]] =>
-            rewrite (proj1 (bound_var_ctx_comp_ctx))
-        end | normalize_bound_var_ctx'].
-
-  Ltac  normalize_bound_var_ctx_in_ctx :=
-    first [
-        match goal with
-          | [H:context[bound_var_ctx (comp_ctx_f _ _)] |- _] =>
-            rewrite (proj2 (bound_var_ctx_comp_ctx)) in H
-          | [H:context [bound_var_fundefs_ctx (comp_f_ctx_f _ _)] |- _] =>
-            rewrite (proj2 (bound_var_ctx_comp_ctx)) in H
-        end| normalize_bound_var_ctx_in_ctx'].
-
 
   Theorem sig_inv_full_dead:
     forall c c' e sig,
@@ -2680,21 +2362,9 @@ Section CONTRACT.
   Definition closed_fundefs :=
     fun f => Empty_set var <--> occurs_free_fundefs f.
 
-  Theorem Decidable_name_in_fundefs_ctx :
-    forall cf, Decidable (name_in_fundefs_ctx cf).
-  Proof.
-    induction cf; simpl.
-    apply Decidable_Union.
-    apply Decidable_singleton_var.
-    apply Decidable_name_in_fundefs.
-    apply Decidable_Union.
-    apply Decidable_singleton_var.
-    auto.
-  Qed.         
-
   Theorem fun_names_not_free_in_fundefs_ctx :
     forall x f7,
-      name_in_fundefs_ctx f7 x
+      names_in_fundefs_ctx f7 x
       -> ~ occurs_free_fundefs_ctx f7 x.
   Proof.
     induction f7; intros; intro.
@@ -2972,7 +2642,7 @@ Section CONTRACT.
   
   
   Theorem name_in_bound_var_fundefs_ctx: forall cf,
-                                           Included _ (name_in_fundefs_ctx cf) (bound_var_fundefs_ctx cf).
+                                           Included _ (names_in_fundefs_ctx cf) (bound_var_fundefs_ctx cf).
   Proof.
     induction cf; simpl; normalize_bound_var_ctx; auto with Ensembles_DB.
     intro. intro. inv H. auto.
@@ -4086,7 +3756,7 @@ Section CONTRACT.
 
   Theorem name_in_fundefs_ctx_rename_all_ns:
     forall sig f,
-      name_in_fundefs_ctx f <--> name_in_fundefs_ctx (rename_all_fun_ctx_ns sig f).
+      names_in_fundefs_ctx f <--> names_in_fundefs_ctx (rename_all_fun_ctx_ns sig f).
   Proof.
     induction f; simpl; eauto with Ensembles_DB.
     rewrite name_in_fundefs_rename_all_ns. reflexivity. 
@@ -4171,7 +3841,7 @@ Section CONTRACT.
         bound_stem_ctx c x) /\
     ( forall fds,
         ~ occurs_free_fundefs (fds <[e]>) x ->
-        bound_stem_fundefs_ctx fds x \/ name_in_fundefs_ctx fds x).
+        bound_stem_fundefs_ctx fds x \/ names_in_fundefs_ctx fds x).
   Proof.
     intro H.
     apply exp_fundefs_ctx_mutual_ind; intros.
@@ -4209,14 +3879,14 @@ Section CONTRACT.
       destruct Hv. specialize (Dec x). destruct Dec.
       constructor.
       auto.
-      apply Bound_Fun12_c. apply H0. intro.
+      apply SBound_Fun12_c. apply H0. intro.
       apply H1.
       apply Free_Efun1; auto.
     + simpl in H1.
       assert (Hv := Decidable_name_in_fundefs_ctx f5).
       inv Hv. specialize (Dec x). inv Dec.
       constructor; auto.
-      apply Bound_Fun2_c.
+      apply SBound_Fun2_c.
       assert (~ occurs_free_fundefs (f5 <[ e ]>) x).
       intro.
       apply H1.
@@ -4232,7 +3902,7 @@ Section CONTRACT.
       assert (Hl := Decidable_FromList l).
       inv Hl. specialize (Dec x). inv Dec. 
       constructor. auto.
-      apply Bound_Fcons12_c. apply H0. intro. apply H1.
+      apply SBound_Fcons12_c. apply H0. intro. apply H1.
       constructor; auto. intro. apply H2. subst; constructor.
       constructor.
       intro; apply H2. constructor 2. auto.
@@ -5420,49 +5090,6 @@ Section CONTRACT.
 
   
   (* TODO: move to identifiers *)
-  Lemma bound_stem_ctx_dec_mut :
-    (forall c, Decidable (bound_stem_ctx c)) /\
-    (forall Bc, Decidable (bound_stem_fundefs_ctx Bc)).
-  Proof.
-    exp_fundefs_ctx_induction IHc IHf; split; intro x; try (inv IHc; specialize (Dec x); inv Dec; auto);
-    try (inv IHf; specialize (Dec x); inv Dec; auto).
-    - right; intro; inv H.
-    - destruct (var_dec v x); subst; auto.
-      right; intro Hbv; inv Hbv; auto.
-    - destruct (var_dec v x); subst; auto.
-      right; intro Hbv; inv Hbv; auto.
-    - destruct (var_dec v x); subst; auto.
-      right; intro Hbv; inv Hbv; auto.
-    - right. intro. apply H. inv H0. auto.
-    - 
-      assert (Hn := Decidable_name_in_fundefs f4).
-      inv Hn. specialize (Dec x). inv Dec.
-      left; auto. 
-      right. intro. apply H. inv H1. exfalso; auto. auto.
-    -
-      assert (Hf5 := Decidable_name_in_fundefs_ctx f5). inv Hf5. specialize (Dec x). inv Dec.
-      left.
-      constructor. auto.
-      right. intro; apply H. inv H1.
-      exfalso; auto. auto.
-    -  destruct (in_dec var_dec x l); auto.
-       right; intro. apply H. inv H0. exfalso; auto. auto.
-    - right.
-      intro; apply H. inv H0. auto.
-  Qed.
-
-  Lemma bound_stem_ctx_dec:
-    (forall c, Decidable (bound_stem_ctx c)).
-  Proof.
-    intro. apply bound_stem_ctx_dec_mut.
-  Qed.
-
-
-  Lemma bound_stem_fundefs_ctx_dec:
-    (forall c, Decidable (bound_stem_fundefs_ctx c)).
-  Proof.
-    intro. apply bound_stem_ctx_dec_mut.
-  Qed.
 
 
 
@@ -5530,245 +5157,13 @@ Section CONTRACT.
     - simpl in H. inv H. intro. intro. auto.
   Qed.
   
-  (* variables bound NOT  on the way to the hole *)
-  Inductive bound_not_stem_ctx: exp_ctx -> Ensemble var  :=
-  | NBound_Constr_c: forall c v v' t ys,
-                       bound_not_stem_ctx c v ->
-                       bound_not_stem_ctx (Econstr_c v' t ys c) v
-  | NBound_Proj_c: forall  t n r c v' v,
-                     bound_not_stem_ctx c v' ->
-                     bound_not_stem_ctx (Eproj_c v t n r c) v'
-  | NBound_Prim_c: forall  t r c v' v,
-                     bound_not_stem_ctx c v' ->
-                     bound_not_stem_ctx (Eprim_c v t r c) v'
-  | NBound_Case2_c: forall v v' e lce t' t c lce',
-                      bound_var e v' ->
-                      List.In (t',e) lce ->
-                      bound_not_stem_ctx (Ecase_c v lce t c lce') v'
-  | NBound_Case3_c: forall v v' e lce t' t c lce',
-                      bound_var e v' ->
-                      List.In (t',e) lce' ->
-                      bound_not_stem_ctx (Ecase_c v lce t c lce') v'
-  | NBound_Case1_c: forall v v' lce t c lce',
-                      bound_not_stem_ctx c v' ->
-                      bound_not_stem_ctx (Ecase_c v lce t c lce') v'
-  | NBound_Fun11_c: forall fds v c,
-                      ~ name_in_fundefs fds v ->
-                      bound_var_fundefs fds v ->
-                      bound_not_stem_ctx (Efun1_c fds c) v
-  | NBound_Fun12_c: forall fds v c,
-                      bound_not_stem_ctx c v ->
-                      bound_not_stem_ctx (Efun1_c fds c) v
-  | NBound_Fun1_c: forall cfds v e,
-                     bound_not_stem_fundefs_ctx cfds v ->
-                     bound_not_stem_ctx (Efun2_c cfds e) v
-  | NBound_Fun2_c: forall cfds e v,
-                     bound_var e v ->
-                     bound_not_stem_ctx (Efun2_c cfds e) v
-  with bound_not_stem_fundefs_ctx: fundefs_ctx -> Ensemble var :=
-       | NBound_Fcons11_c: forall f t xs c fds v,
-                             bound_not_stem_ctx c v ->
-                             bound_not_stem_fundefs_ctx (Fcons1_c f t xs c fds) v
-       | NBound_Fcons12_c: forall f t xs c fds v,
-                             ~ name_in_fundefs fds v ->
-                             bound_var_fundefs fds v ->
-                             bound_not_stem_fundefs_ctx (Fcons1_c f t xs c fds) v
-       | NBound_Fcons21_c: forall f t xs e cfds v,
-                             bound_not_stem_fundefs_ctx cfds v ->
-                             bound_not_stem_fundefs_ctx (Fcons2_c f t xs e cfds) v
-       | NBound_Fcons22_c: forall f t xs e cfds v,
-                             bound_var e v ->
-                             bound_not_stem_fundefs_ctx (Fcons2_c f t xs e cfds) v
-       | NBound_Fcons23_c:
-           forall f t xs e cfds v,
-             FromList xs v ->
-             bound_not_stem_fundefs_ctx (Fcons2_c f t xs e cfds) v
-  .
 
 
   Hint Constructors bound_not_stem_ctx.
   Hint Constructors bound_not_stem_fundefs_ctx.
 
 
-  Lemma bound_not_stem_Econstr_c x t ys c :
-    Same_set _ (bound_not_stem_ctx (Econstr_c x t ys c))
-             (bound_not_stem_ctx c).
-  Proof.
-    
-    split; intros x' H;  eauto. inv H; eauto.
-  Qed.
 
-  Lemma bound_not_stem_Eproj_c v t n r c :
-    Same_set _ (bound_not_stem_ctx (Eproj_c v t n r c))
-             (bound_not_stem_ctx c).
-  Proof.
-    split; intros x' H; auto.  inv H; auto.
-  Qed.
-
-  Lemma bound_not_stem_Eprim_c x tau y c :
-    Same_set _ (bound_not_stem_ctx (Eprim_c x tau y c))
-             (bound_not_stem_ctx c).
-  Proof.
-    split; intros x' H; auto. inv H; auto.  
-  Qed.
-
-  Lemma bound_not_stem_Hole_c :
-    Same_set _ (bound_not_stem_ctx Hole_c)
-             (Empty_set var).
-  Proof.
-    split; intros x' H; inv H; eauto. 
-  Qed.
-
-  Lemma bound_not_stem_Case_c :
-    forall v  lce t c lce',
-      Same_set _ (bound_not_stem_ctx (Ecase_c v lce t c lce'))
-               (Union _ (bound_not_stem_ctx c) (Union _ (bound_var (Ecase v lce))
-                                                      (bound_var (Ecase v lce')))).
-  Proof with eauto with Ensembles_DB.
-    split; intros; intro; intros.
-    - inversion H; subst; eauto.
-    - inv H; auto.
-      inv H0. inv H.
-      eapply NBound_Case2_c; eauto.
-      inv H.
-      eapply NBound_Case3_c; eauto.
-  Qed.
-
-
-  Lemma bound_not_stem_Fun1_c :
-    forall fds c,
-      Same_set _ (bound_not_stem_ctx (Efun1_c fds c))
-               (Union _ (Setminus _ (bound_var_fundefs fds) (name_in_fundefs fds)) (bound_not_stem_ctx c)).
-  Proof.
-    split; intros x H; inv H; auto.
-    left. split; auto.
-    inv H0. auto.
-  Qed.
-
-  Lemma bound_not_stem_Fun2_c :
-    forall cfds e,
-      Same_set _ (bound_not_stem_ctx (Efun2_c cfds e))
-               (Union _ (bound_var e) (bound_not_stem_fundefs_ctx cfds)).
-  Proof.
-    split; intros x H; inv H; eauto.
-  Qed.
-
-  Lemma bound_not_stem_Fcons1_c :
-    forall c v l e0 f,
-      Same_set _ (bound_not_stem_fundefs_ctx (Fcons1_c v c l e0 f))
-               (Union _ (bound_not_stem_ctx e0) (Setminus _ (bound_var_fundefs f) (name_in_fundefs f))).             
-  Proof.
-    split; intros x H; auto.
-    inv H. auto. right; split; auto.
-    inv H; auto. inv H0; auto. 
-  Qed.  
-
-  Lemma bound_not_stem_Fcons2_c :
-    forall c v l e0 f,
-      Same_set _ (bound_not_stem_fundefs_ctx (Fcons2_c v c l e0 f))
-               (Union _ (Union _ (bound_var e0) (FromList l)) (bound_not_stem_fundefs_ctx f)).             
-  Proof.
-    split; intros x H; inv H; eauto.
-    inv H0; auto.
-  Qed.  
-
-  Ltac normalize_bound_not_stem_ctx' :=
-    match goal with
-      | [ |- context[bound_not_stem_ctx Hole_c]] =>
-        rewrite bound_not_stem_Hole_c 
-      | [|- context[bound_not_stem_ctx (Econstr_c _ _ _ _)]] =>
-        rewrite bound_not_stem_Econstr_c
-      | [|- context[bound_not_stem_ctx (Eproj_c _ _ _ _ _)]] =>
-        rewrite bound_not_stem_Eproj_c
-      | [|- context[bound_not_stem_ctx (Ecase_c _ _ _ _ _)]] =>
-        rewrite bound_not_stem_Case_c
-      | [ |- context[bound_not_stem_ctx (Efun1_c _ _)]] =>
-        rewrite bound_not_stem_Fun1_c 
-      | [ |- context[bound_not_stem_ctx (Efun2_c _ _)] ] =>
-        rewrite bound_not_stem_Fun2_c
-      | [|- context[bound_not_stem_ctx (Eprim_c _ _ _ _)]] =>
-        rewrite bound_not_stem_Eprim_c
-      | [|- context[bound_not_stem_fundefs_ctx (Fcons1_c _ _ _ _ _)]] =>
-        rewrite bound_not_stem_Fcons1_c
-      | [|- context[bound_not_stem_fundefs_ctx (Fcons2_c _ _ _ _ _)]] =>
-        rewrite bound_not_stem_Fcons2_c
-    end.
-
-  Ltac normalize_bound_not_stem_ctx_in_ctx' :=
-    match goal with
-      | [ H: context[bound_not_stem_ctx Hole_c] |- _] =>
-        rewrite bound_not_stem_Hole_c in H
-      | [ H : context[bound_not_stem_ctx (Econstr_c _ _ _ _)] |- _ ] =>
-        rewrite bound_not_stem_Econstr_c in H
-      | [ H : context[bound_not_stem_ctx (Eproj_c _ _ _ _ _)]  |- _ ] =>
-        rewrite bound_not_stem_Eproj_c in H
-      | [H: context[bound_not_stem_ctx (Ecase_c _ _ _ _ _)] |- _] =>
-        rewrite bound_not_stem_Case_c in H
-      | [ H : context[bound_not_stem_ctx (Efun1_c _ _)] |- _ ] =>
-        rewrite bound_not_stem_Fun1_c in H
-      | [ H : context[bound_not_stem_ctx (Efun2_c _ _)] |- _ ] =>
-        rewrite bound_not_stem_Fun2_c in H
-      | [ H : context[bound_not_stem_ctx (Eprim_c _ _ _ _)] |- _ ] =>
-        rewrite bound_not_stem_Eprim_c in H
-      | [H:context[bound_not_stem_fundefs_ctx (Fcons1_c _ _ _ _ _)] |- _] =>
-        rewrite bound_not_stem_Fcons1_c in H
-      | [H: context[bound_not_stem_fundefs_ctx (Fcons2_c _ _ _ _ _)] |- _] =>
-        rewrite bound_not_stem_Fcons2_c in H
-    end.
-
-
-
-
-  Theorem bound_var_stem_or_not_stem_mut:
-    (forall c,
-       Same_set _ (bound_var_ctx c) (Union _ (bound_not_stem_ctx c) (bound_stem_ctx c) ))/\
-    (forall f, Same_set _ (bound_var_fundefs_ctx f) (Union _ (name_in_fundefs_ctx f) (Union _ (bound_not_stem_fundefs_ctx f) (bound_stem_fundefs_ctx f)))).
-  Proof. 
-    apply exp_fundefs_ctx_mutual_ind; intros; try normalize_bound_var_ctx; try normalize_bound_stem_ctx'; try normalize_bound_not_stem_ctx'; try rewrite H; eauto 25 with Ensembles_DB.
-    - split; eauto 25 with Ensembles_DB.
-    - assert (Hn := Decidable_name_in_fundefs f4).
-      split; intro; intros. inv H0; eauto 25 with Ensembles_DB.
-      inv Hn. specialize (Dec x). inv Dec; eauto. left. left. split; auto.
-      inv H1; eauto with Ensembles_DB.
-      inv H0. inv H1. inv H0; auto.
-      auto. inv H1; auto.
-      apply name_in_fundefs_bound_var_fundefs in H0. auto.
-    - split; intro; intros H0; inv H0; eauto 25 with Ensembles_DB.
-      inv H1; auto. inv H0; auto. inv H1; auto. inv H1; auto.
-    - assert (Hf6 := Decidable_name_in_fundefs f6).
-      split; intro; intros H0. inv H0.
-      left; constructor; auto.
-      inv H1. right; right; auto.
-      inv H0; auto. inv H1; auto.
-      inv Hf6. specialize (Dec x). inv Dec. left. constructor 2; auto.
-      right. left. right.  split; auto.
-      inv H0. inv H1. auto. apply name_in_fundefs_bound_var_fundefs in H0. auto.
-      inv H1; auto. inv H0; auto. inv H1. auto.
-      inv H0; auto.
-    - split; intro; intros H0; inv H0; eauto 25 with Ensembles_DB.
-      left; constructor; auto.
-      inv H1; auto. inv H0; auto. inv H1; auto. left; constructor 2; auto.
-      inv H0; auto.
-      inv H1; auto.
-      inv H1; auto. inv H0; auto. inv H1; auto. right. right. right. auto.
-      right. right. right. auto.
-  Qed.
-
-
-  Theorem bound_var_stem_or_not_stem:
-    forall c,
-      Same_set _ (bound_var_ctx c) (Union _ (bound_not_stem_ctx c) (bound_stem_ctx c)).       
-  Proof. 
-    intros.
-    apply bound_var_stem_or_not_stem_mut.
-  Qed.
-  
-  Theorem bound_var_fundefs_stem_or_not_stem:
-    (forall f, Same_set _ (bound_var_fundefs_ctx f) (Union _ (name_in_fundefs_ctx f) (Union _ (bound_not_stem_fundefs_ctx f) (bound_stem_fundefs_ctx f)))).
-  Proof.
-    intro.
-    apply bound_var_stem_or_not_stem_mut.
-  Qed.
 
 
   Theorem Proper_Intersection:
@@ -5785,7 +5180,7 @@ Section CONTRACT.
   Theorem ub_disjoint_name_not_stem_ctx:
     forall f5,
       unique_bindings_fundefs_c f5 ->
-      Disjoint _ (name_in_fundefs_ctx f5) (bound_not_stem_fundefs_ctx f5).
+      Disjoint _ (names_in_fundefs_ctx f5) (bound_not_stem_fundefs_ctx f5).
   Proof.
     induction f5; intros; simpl; try normalize_bound_not_stem_ctx'.
     - inv H.
@@ -6343,7 +5738,7 @@ Section CONTRACT.
   
   Theorem bound_var_fundefs_ctx_append_f:
     forall im fdc,
-      Included _ (name_in_fundefs_ctx fdc)
+      Included _ (names_in_fundefs_ctx fdc)
                (bound_var_fundefs_ctx (inlined_fundefs_ctx_f fdc im)).
   Proof.
     induction fdc.
@@ -6360,7 +5755,7 @@ Section CONTRACT.
   
   Theorem name_in_fundefs_ctx_append:
     forall fdc fds,
-      Same_set _ (name_in_fundefs_ctx (fundefs_ctx_append fds fdc)) (Union _ (name_in_fundefs fds) (name_in_fundefs_ctx fdc)).
+      Same_set _ (names_in_fundefs_ctx (fundefs_ctx_append fds fdc)) (Union _ (name_in_fundefs fds) (names_in_fundefs_ctx fdc)).
   Proof.
     induction fds.
     - simpl. rewrite IHfds; auto with Ensembles_DB.
@@ -7990,23 +7385,21 @@ Section CONTRACT.
           - left.
             apply num_occur_app_ctx in H12.  destruct H12. destruct H12. inversion H12.
             inversion H14. pi0.
-            apply plus_is_O in H16.
-            inversion H16.
-            clear H14. clear H12.
-            clear H16. rewrite H17 in *.
-            rewrite H18 in *.
+            destruct H14.
+            clear H14.
+            clear H16.
             rewrite He1 in H15.
             clear He1.
             subst.
             repeat normalize_ctx.
             apply num_occur_ec_comp_ctx in H13.
             destructAll; pi0.
-            simpl in H13. inv H13; pi0.
-            rewrite inlined_fundefs_ctx_append_shallow in H20.
-            rewrite rename_all_fundefs_ctx_append in H20.
-            apply fundefs_ctx_append_num_occur' in H20.
+            simpl in H17. inv H17; pi0.
+            rewrite inlined_fundefs_ctx_append_shallow in H24.
+            rewrite rename_all_fundefs_ctx_append in H24.
+            apply fundefs_ctx_append_num_occur' in H24.
             destructAll; pi0.
-            simpl in H14.  inv H14; pi0.
+            simpl in H18.  inv H18; pi0.
             apply num_occur_app_ctx. exists 0, 0.
             split; auto.
             apply num_occur_ec_comp_ctx.
@@ -8023,7 +7416,7 @@ Section CONTRACT.
             rewrite rename_all_ns_fundefs_append.
             eapply fundefs_append_num_occur.
             reflexivity.
-            rewrite rename_all_fun_ns_inlined_fundefs in H13.
+            rewrite rename_all_fun_ns_inlined_fundefs in H17.
             rewrite rename_all_fun_ns_inlined_fundefs.
             eapply dead_occur_fds_le_antimon. simpl in b.
             apply b_map_le_c. eauto. auto.
@@ -8031,7 +7424,7 @@ Section CONTRACT.
             simpl. constructor. simpl. eapply num_occur_fds_n.
             constructor. eauto. constructor.
             auto.
-            rewrite rename_all_fun_ns_inlined_fundefs in H25.
+            rewrite rename_all_fun_ns_inlined_fundefs in H29.
             rewrite rename_all_fun_ns_inlined_fundefs.
             eapply dead_occur_fds_le_antimon. simpl in b.
             apply b_map_le_c. eauto. auto.
