theories/L6_PCPS/stemctx.v
@@ -1,0 +1,518 @@
+(* Library extending ctx with a notion of bound on the stem of a context, as used in the proof of correctness of the shrink inliner *)
+
+Require Import Coq.Lists.List Coq.Lists.SetoidList Coq.NArith.BinNat Coq.PArith.BinPos
+        Coq.MSets.MSetRBT Coq.Lists.List Coq.Sets.Ensembles Omega Coq.Sorting.Permutation.
+Require Import Libraries.Coqlib.
+Require Import L6.cps L6.cps_util L6.ctx L6.set_util L6.Ensembles_util L6.List_util L6.size_cps L6.identifiers.
+Import ListNotations.
+
+(** bound_stem_ctx is the set of the variables bound on the stem of a context (from the root to the hole) *)
+  Inductive bound_stem_ctx: exp_ctx -> Ensemble var  :=
+  | SBound_Constr1_c: forall v t ys c,
+                       bound_stem_ctx (Econstr_c v t ys c) v
+  | SBound_Constr2_c: forall c v v' t ys,
+                       bound_stem_ctx c v ->
+                       bound_stem_ctx (Econstr_c v' t ys c) v
+  | SBound_Proj1_c: forall  t n r c v,
+                     bound_stem_ctx (Eproj_c v t n r c) v
+  | SBound_Proj2_c: forall  t n r c v' v,
+                     bound_stem_ctx c v' ->
+                     bound_stem_ctx (Eproj_c v t n r c) v'
+  | SBound_Prim1_c: forall  x f ys c,
+                     bound_stem_ctx (Eprim_c x f ys c) x
+  | SBound_Prim2_c: forall  t r c v' v,
+                     bound_stem_ctx c v' ->
+                     bound_stem_ctx (Eprim_c v t r c) v'
+  | SBound_Case1_c: forall v v' lce t c lce',
+                     bound_stem_ctx c v' ->
+                     bound_stem_ctx (Ecase_c v lce t c lce') v'
+  | SBound_Fun11_c: forall fds v c,
+                     name_in_fundefs fds v ->
+                     bound_stem_ctx (Efun1_c fds c) v
+  | SBound_Fun12_c: forall fds v c,
+                     bound_stem_ctx c v ->
+                     bound_stem_ctx (Efun1_c fds c) v
+  | SBound_Fun21_c: forall fds v c,
+                     names_in_fundefs_ctx fds v ->
+                     bound_stem_ctx (Efun2_c fds c) v 
+
+  | SBound_Fun2_c: forall cfds v e,
+                    bound_stem_fundefs_ctx cfds v ->
+                    bound_stem_ctx (Efun2_c cfds e) v
+  with bound_stem_fundefs_ctx: fundefs_ctx -> Ensemble var :=
+                                                  | SBound_Fcons11_c: forall f t xs c fds v,
+                                                                       List.In v xs ->
+                                                                       bound_stem_fundefs_ctx (Fcons1_c f t xs c fds) v
+
+                                                  | SBound_Fcons12_c: forall f t xs c fds v,
+                                                                       bound_stem_ctx c v ->
+                                                                       bound_stem_fundefs_ctx (Fcons1_c f t xs c fds) v
+                                                  | SBound_Fcons2_c: forall f t xs e cfds v,
+                                                                      bound_stem_fundefs_ctx cfds v ->
+                                                                      bound_stem_fundefs_ctx (Fcons2_c f t xs e cfds) v.
+
+  Hint Constructors bound_stem_ctx.
+  Hint Constructors bound_stem_fundefs_ctx.
+
+
+  Lemma bound_stem_Econstr_c x t ys c :
+    Same_set _ (bound_stem_ctx (Econstr_c x t ys c))
+             (Union var (bound_stem_ctx c) (Singleton _ x)).
+  Proof.
+    split; intros x' H; inv H; eauto. inv H0; eauto.
+  Qed.
+
+  Lemma bound_stem_Eproj_c v t n r c :
+    Same_set _ (bound_stem_ctx (Eproj_c v t n r c))
+             (Union var (bound_stem_ctx c) (Singleton _ v)).
+  Proof.
+    split; intros x' H; inv H; eauto. inv H0; eauto.
+  Qed.
+
+  Lemma bound_stem_Eprim_c x tau y c :
+    Same_set _ (bound_stem_ctx (Eprim_c x tau y c))
+             (Union var (bound_stem_ctx c) (Singleton _ x)).
+  Proof.
+    split; intros x' H; inv H; eauto. inv H0; eauto.
+  Qed.
+
+  Lemma bound_stem_Hole_c :
+    Same_set _ (bound_stem_ctx Hole_c)
+             (Empty_set var).
+  Proof.
+    split; intros x' H; inv H; eauto. 
+  Qed.
+
+  Lemma bound_stem_Case_c :
+    forall v  lce t c lce',
+      Same_set _ (bound_stem_ctx (Ecase_c v lce t c lce'))
+               (bound_stem_ctx c).
+  Proof with eauto with Ensembles_DB.
+    split; intros; intro; intros.
+    - inversion H; subst; eauto.
+    - constructor.
+      auto.
+  Qed.
+
+
+  Lemma bound_stem_Fun1_c :
+    forall fds c,
+      Same_set _ (bound_stem_ctx (Efun1_c fds c))
+               (Union _ (name_in_fundefs fds) (bound_stem_ctx c)).
+  Proof.
+    split; intros x H; inv H; eauto.
+  Qed.
+
+  Lemma bound_stem_Fun2_c :
+    forall cfds e,
+      Same_set _ (bound_stem_ctx (Efun2_c cfds e))
+               (Union _ (names_in_fundefs_ctx cfds) (bound_stem_fundefs_ctx cfds)).
+  Proof.
+    split; intros x H; inv H; eauto.
+  Qed.
+
+  Lemma bound_stem_Fcons1_c :
+    forall c v l e0 f,
+      Same_set _ (bound_stem_fundefs_ctx (Fcons1_c v c l e0 f))
+               (Union _ (bound_stem_ctx e0) (FromList l)).             
+  Proof.
+    split; intros x H; inv H; eauto.
+  Qed.  
+
+  Lemma bound_stem_Fcons2_c :
+    forall c v l e0 f,
+      Same_set _ (bound_stem_fundefs_ctx (Fcons2_c v c l e0 f))
+               (bound_stem_fundefs_ctx f).             
+  Proof.
+    split; intros x H; inv H; eauto.
+  Qed.
+
+
+  Ltac normalize_bound_stem_ctx' :=
+    match goal with
+      | [ |- context[bound_stem_ctx Hole_c]] =>
+        rewrite bound_stem_Hole_c 
+      | [|- context[bound_stem_ctx (Econstr_c _ _ _ _)]] =>
+        rewrite bound_stem_Econstr_c
+      | [|- context[bound_stem_ctx (Eproj_c _ _ _ _ _)]] =>
+        rewrite bound_stem_Eproj_c
+      | [|- context[bound_stem_ctx (Ecase_c _ _ _ _ _)]] =>
+        rewrite bound_stem_Case_c
+      | [ |- context[bound_stem_ctx (Efun1_c _ _)]] =>
+        rewrite bound_stem_Fun1_c 
+      | [ |- context[bound_stem_ctx (Efun2_c _ _)] ] =>
+        rewrite bound_stem_Fun2_c
+      | [|- context[bound_stem_ctx (Eprim_c _ _ _ _)]] =>
+        rewrite bound_stem_Eprim_c
+      | [|- context[bound_stem_fundefs_ctx (Fcons1_c _ _ _ _ _)]] =>
+        rewrite bound_stem_Fcons1_c
+      | [|- context[bound_stem_fundefs_ctx (Fcons2_c _ _ _ _ _)]] =>
+        rewrite bound_stem_Fcons2_c
+    end.
+
+  Ltac normalize_bound_stem_ctx_in_ctx' :=
+    match goal with
+      | [ H: context[bound_stem_ctx Hole_c] |- _] =>
+        rewrite bound_stem_Hole_c in H
+      | [ H : context[bound_stem_ctx (Econstr_c _ _ _ _)] |- _ ] =>
+        rewrite bound_stem_Econstr_c in H
+      | [ H : context[bound_stem_ctx (Eproj_c _ _ _ _ _)]  |- _ ] =>
+        rewrite bound_stem_Eproj_c in H
+      | [H: context[bound_stem_ctx (Ecase_c _ _ _ _ _)] |- _] =>
+        rewrite bound_stem_Case_c in H
+      | [ H : context[bound_stem_ctx (Efun1_c _ _)] |- _ ] =>
+        rewrite bound_stem_Fun1_c in H
+      | [ H : context[bound_stem_ctx (Efun2_c _ _)] |- _ ] =>
+        rewrite bound_stem_Fun2_c in H
+      | [ H : context[bound_stem_ctx (Eprim_c _ _ _ _)] |- _ ] =>
+        rewrite bound_stem_Eprim_c in H
+      | [H:context[bound_stem_fundefs_ctx (Fcons1_c _ _ _ _ _)] |- _] =>
+        rewrite bound_stem_Fcons1_c in H
+      | [H: context[bound_stem_fundefs_ctx (Fcons2_c _ _ _ _ _)] |- _] =>
+        rewrite bound_stem_Fcons2_c in H
+    end.
+
+
+
+
+
+    (* variables bound NOT  on the way to the hole *)
+  Inductive bound_not_stem_ctx: exp_ctx -> Ensemble var  :=
+  | NBound_Constr_c: forall c v v' t ys,
+                       bound_not_stem_ctx c v ->
+                       bound_not_stem_ctx (Econstr_c v' t ys c) v
+  | NBound_Proj_c: forall  t n r c v' v,
+                     bound_not_stem_ctx c v' ->
+                     bound_not_stem_ctx (Eproj_c v t n r c) v'
+  | NBound_Prim_c: forall  t r c v' v,
+                     bound_not_stem_ctx c v' ->
+                     bound_not_stem_ctx (Eprim_c v t r c) v'
+  | NBound_Case2_c: forall v v' e lce t' t c lce',
+                      bound_var e v' ->
+                      List.In (t',e) lce ->
+                      bound_not_stem_ctx (Ecase_c v lce t c lce') v'
+  | NBound_Case3_c: forall v v' e lce t' t c lce',
+                      bound_var e v' ->
+                      List.In (t',e) lce' ->
+                      bound_not_stem_ctx (Ecase_c v lce t c lce') v'
+  | NBound_Case1_c: forall v v' lce t c lce',
+                      bound_not_stem_ctx c v' ->
+                      bound_not_stem_ctx (Ecase_c v lce t c lce') v'
+  | NBound_Fun11_c: forall fds v c,
+                      ~ name_in_fundefs fds v ->
+                      bound_var_fundefs fds v ->
+                      bound_not_stem_ctx (Efun1_c fds c) v
+  | NBound_Fun12_c: forall fds v c,
+                      bound_not_stem_ctx c v ->
+                      bound_not_stem_ctx (Efun1_c fds c) v
+  | NBound_Fun1_c: forall cfds v e,
+                     bound_not_stem_fundefs_ctx cfds v ->
+                     bound_not_stem_ctx (Efun2_c cfds e) v
+  | NBound_Fun2_c: forall cfds e v,
+                     bound_var e v ->
+                     bound_not_stem_ctx (Efun2_c cfds e) v
+  with bound_not_stem_fundefs_ctx: fundefs_ctx -> Ensemble var :=
+       | NBound_Fcons11_c: forall f t xs c fds v,
+                             bound_not_stem_ctx c v ->
+                             bound_not_stem_fundefs_ctx (Fcons1_c f t xs c fds) v
+       | NBound_Fcons12_c: forall f t xs c fds v,
+                             ~ name_in_fundefs fds v ->
+                             bound_var_fundefs fds v ->
+                             bound_not_stem_fundefs_ctx (Fcons1_c f t xs c fds) v
+       | NBound_Fcons21_c: forall f t xs e cfds v,
+                             bound_not_stem_fundefs_ctx cfds v ->
+                             bound_not_stem_fundefs_ctx (Fcons2_c f t xs e cfds) v
+       | NBound_Fcons22_c: forall f t xs e cfds v,
+                             bound_var e v ->
+                             bound_not_stem_fundefs_ctx (Fcons2_c f t xs e cfds) v
+       | NBound_Fcons23_c:
+           forall f t xs e cfds v,
+             FromList xs v ->
+             bound_not_stem_fundefs_ctx (Fcons2_c f t xs e cfds) v
+  .
+
+  
+  Hint Constructors bound_not_stem_ctx.
+  Hint Constructors bound_not_stem_fundefs_ctx.
+
+    Lemma bound_not_stem_Econstr_c x t ys c :
+    Same_set _ (bound_not_stem_ctx (Econstr_c x t ys c))
+             (bound_not_stem_ctx c).
+  Proof.
+    
+    split; intros x' H;  eauto. inv H; eauto.
+  Qed.
+
+  Lemma bound_not_stem_Eproj_c v t n r c :
+    Same_set _ (bound_not_stem_ctx (Eproj_c v t n r c))
+             (bound_not_stem_ctx c).
+  Proof.
+    split; intros x' H; auto.  inv H; auto.
+  Qed.
+
+  Lemma bound_not_stem_Eprim_c x tau y c :
+    Same_set _ (bound_not_stem_ctx (Eprim_c x tau y c))
+             (bound_not_stem_ctx c).
+  Proof.
+    split; intros x' H; auto. inv H; auto.  
+  Qed.
+
+  Lemma bound_not_stem_Hole_c :
+    Same_set _ (bound_not_stem_ctx Hole_c)
+             (Empty_set var).
+  Proof.
+    split; intros x' H; inv H; eauto. 
+  Qed.
+
+  Lemma bound_not_stem_Case_c :
+    forall v  lce t c lce',
+      Same_set _ (bound_not_stem_ctx (Ecase_c v lce t c lce'))
+               (Union _ (bound_not_stem_ctx c) (Union _ (bound_var (Ecase v lce))
+                                                      (bound_var (Ecase v lce')))).
+  Proof with eauto with Ensembles_DB.
+    split; intros; intro; intros.
+    - inversion H; subst; eauto.
+    - inv H; auto.
+      inv H0. inv H.
+      eapply NBound_Case2_c; eauto.
+      inv H.
+      eapply NBound_Case3_c; eauto.
+  Qed.
+
+
+  Lemma bound_not_stem_Fun1_c :
+    forall fds c,
+      Same_set _ (bound_not_stem_ctx (Efun1_c fds c))
+               (Union _ (Setminus _ (bound_var_fundefs fds) (name_in_fundefs fds)) (bound_not_stem_ctx c)).
+  Proof.
+    split; intros x H; inv H; auto.
+    left. split; auto.
+    inv H0. auto.
+  Qed.
+
+  Lemma bound_not_stem_Fun2_c :
+    forall cfds e,
+      Same_set _ (bound_not_stem_ctx (Efun2_c cfds e))
+               (Union _ (bound_var e) (bound_not_stem_fundefs_ctx cfds)).
+  Proof.
+    split; intros x H; inv H; eauto.
+  Qed.
+
+  Lemma bound_not_stem_Fcons1_c :
+    forall c v l e0 f,
+      Same_set _ (bound_not_stem_fundefs_ctx (Fcons1_c v c l e0 f))
+               (Union _ (bound_not_stem_ctx e0) (Setminus _ (bound_var_fundefs f) (name_in_fundefs f))).             
+  Proof.
+    split; intros x H; auto.
+    inv H. auto. right; split; auto.
+    inv H; auto. inv H0; auto. 
+  Qed.  
+
+  Lemma bound_not_stem_Fcons2_c :
+    forall c v l e0 f,
+      Same_set _ (bound_not_stem_fundefs_ctx (Fcons2_c v c l e0 f))
+               (Union _ (Union _ (bound_var e0) (FromList l)) (bound_not_stem_fundefs_ctx f)).             
+  Proof.
+    split; intros x H; inv H; eauto.
+    inv H0; auto.
+  Qed.  
+
+    Ltac normalize_bound_not_stem_ctx' :=
+    match goal with
+      | [ |- context[bound_not_stem_ctx Hole_c]] =>
+        rewrite bound_not_stem_Hole_c 
+      | [|- context[bound_not_stem_ctx (Econstr_c _ _ _ _)]] =>
+        rewrite bound_not_stem_Econstr_c
+      | [|- context[bound_not_stem_ctx (Eproj_c _ _ _ _ _)]] =>
+        rewrite bound_not_stem_Eproj_c
+      | [|- context[bound_not_stem_ctx (Ecase_c _ _ _ _ _)]] =>
+        rewrite bound_not_stem_Case_c
+      | [ |- context[bound_not_stem_ctx (Efun1_c _ _)]] =>
+        rewrite bound_not_stem_Fun1_c 
+      | [ |- context[bound_not_stem_ctx (Efun2_c _ _)] ] =>
+        rewrite bound_not_stem_Fun2_c
+      | [|- context[bound_not_stem_ctx (Eprim_c _ _ _ _)]] =>
+        rewrite bound_not_stem_Eprim_c
+      | [|- context[bound_not_stem_fundefs_ctx (Fcons1_c _ _ _ _ _)]] =>
+        rewrite bound_not_stem_Fcons1_c
+      | [|- context[bound_not_stem_fundefs_ctx (Fcons2_c _ _ _ _ _)]] =>
+        rewrite bound_not_stem_Fcons2_c
+    end.
+
+  Ltac normalize_bound_not_stem_ctx_in_ctx' :=
+    match goal with
+      | [ H: context[bound_not_stem_ctx Hole_c] |- _] =>
+        rewrite bound_not_stem_Hole_c in H
+      | [ H : context[bound_not_stem_ctx (Econstr_c _ _ _ _)] |- _ ] =>
+        rewrite bound_not_stem_Econstr_c in H
+      | [ H : context[bound_not_stem_ctx (Eproj_c _ _ _ _ _)]  |- _ ] =>
+        rewrite bound_not_stem_Eproj_c in H
+      | [H: context[bound_not_stem_ctx (Ecase_c _ _ _ _ _)] |- _] =>
+        rewrite bound_not_stem_Case_c in H
+      | [ H : context[bound_not_stem_ctx (Efun1_c _ _)] |- _ ] =>
+        rewrite bound_not_stem_Fun1_c in H
+      | [ H : context[bound_not_stem_ctx (Efun2_c _ _)] |- _ ] =>
+        rewrite bound_not_stem_Fun2_c in H
+      | [ H : context[bound_not_stem_ctx (Eprim_c _ _ _ _)] |- _ ] =>
+        rewrite bound_not_stem_Eprim_c in H
+      | [H:context[bound_not_stem_fundefs_ctx (Fcons1_c _ _ _ _ _)] |- _] =>
+        rewrite bound_not_stem_Fcons1_c in H
+      | [H: context[bound_not_stem_fundefs_ctx (Fcons2_c _ _ _ _ _)] |- _] =>
+        rewrite bound_not_stem_Fcons2_c in H
+    end.
+
+
+    Theorem bound_var_stem_or_not_stem_mut:
+    (forall c,
+       Same_set _ (bound_var_ctx c) (Union _ (bound_not_stem_ctx c) (bound_stem_ctx c) ))/\
+    (forall f, Same_set _ (bound_var_fundefs_ctx f) (Union _ (names_in_fundefs_ctx f) (Union _ (bound_not_stem_fundefs_ctx f) (bound_stem_fundefs_ctx f)))).
+  Proof. 
+    apply exp_fundefs_ctx_mutual_ind; intros; try normalize_bound_var_ctx; try normalize_bound_stem_ctx'; try normalize_bound_not_stem_ctx'; try rewrite H; eauto 25 with Ensembles_DB.
+    - split; eauto 25 with Ensembles_DB.
+    - assert (Hn := Decidable_name_in_fundefs f4).
+      split; intro; intros. inv H0; eauto 25 with Ensembles_DB.
+      inv Hn. specialize (Dec x). inv Dec; eauto. left. left. split; auto.
+      inv H1; eauto with Ensembles_DB.
+      inv H0. inv H1. inv H0; auto.
+      auto. inv H1; auto.
+      apply name_in_fundefs_bound_var_fundefs in H0. auto.
+    - split; intro; intros H0; inv H0; eauto 25 with Ensembles_DB.
+      inv H1; auto. inv H0; auto. inv H1; auto. inv H1; auto.
+    - assert (Hf6 := Decidable_name_in_fundefs f6).
+      split; intro; intros H0. inv H0.
+      left; constructor; auto.
+      inv H1. right; right; auto.
+      inv H0; auto. inv H1; auto.
+      inv Hf6. specialize (Dec x). inv Dec. left. constructor 2; auto.
+      right. left. right.  split; auto.
+      inv H0. inv H1. auto. apply name_in_fundefs_bound_var_fundefs in H0. auto.
+      inv H1; auto. inv H0; auto. inv H1. auto.
+      inv H0; auto.
+    - split; intro; intros H0; inv H0; eauto 25 with Ensembles_DB.
+      left; constructor; auto.
+      inv H1; auto. inv H0; auto. inv H1; auto. left; constructor 2; auto.
+      inv H0; auto.
+      inv H1; auto.
+      inv H1; auto. inv H0; auto. inv H1; auto. right. right. right. auto.
+      right. right. right. auto.
+  Qed.
+
+  Theorem bound_stem_var:
+    (forall c,
+       Included _ (bound_stem_ctx c) (bound_var_ctx c))
+    /\
+    (forall fc, Included _ (bound_stem_fundefs_ctx fc) (bound_var_fundefs_ctx fc)).
+  Proof.
+    apply exp_fundefs_ctx_mutual_ind; intros; normalize_bound_var_ctx'; normalize_bound_stem_ctx'; eauto with Ensembles_DB.
+    assert (Hf4 := name_in_fundefs_bound_var_fundefs f4).
+    eauto with Ensembles_DB.
+
+    assert (Hf5 := name_in_fundefs_ctx_bound_var_fundefs f5).
+    eauto with Ensembles_DB.
+  Qed.
+
+  
+
+  Theorem bound_var_stem_or_not_stem:
+    forall c,
+      Same_set _ (bound_var_ctx c) (Union _ (bound_not_stem_ctx c) (bound_stem_ctx c)).       
+  Proof. 
+    intros.
+    apply bound_var_stem_or_not_stem_mut.
+  Qed.
+  
+  Theorem bound_var_fundefs_stem_or_not_stem:
+    (forall f, Same_set _ (bound_var_fundefs_ctx f) (Union _ (names_in_fundefs_ctx f) (Union _ (bound_not_stem_fundefs_ctx f) (bound_stem_fundefs_ctx f)))).
+  Proof.
+    intro.
+    apply bound_var_stem_or_not_stem_mut.
+  Qed.
+
+    Theorem bound_stem_app_fundefs_ctx:
+    forall c fd fd' f tau xs,
+      (bound_stem_fundefs_ctx (app_fundefs_ctx fd (Fcons1_c f tau xs c fd'))) <--> (Union _ (bound_stem_ctx c) (FromList xs)) .
+  Proof.
+    induction fd; intros.
+    - simpl.
+      rewrite bound_stem_Fcons2_c. eapply IHfd. 
+    - simpl. rewrite bound_stem_Fcons1_c.
+      reflexivity.
+  Qed.      
+
+  Lemma bound_stem_ctx_dec_mut :
+    (forall c, Decidable (bound_stem_ctx c)) /\
+    (forall Bc, Decidable (bound_stem_fundefs_ctx Bc)).
+  Proof.
+    exp_fundefs_ctx_induction IHc IHf; split; intro x; try (inv IHc; specialize (Dec x); inv Dec; auto);
+    try (inv IHf; specialize (Dec x); inv Dec; auto).
+    - right; intro; inv H.
+    - destruct (var_dec v x); subst; auto.
+      right; intro Hbv; inv Hbv; auto.
+    - destruct (var_dec v x); subst; auto.
+      right; intro Hbv; inv Hbv; auto.
+    - destruct (var_dec v x); subst; auto.
+      right; intro Hbv; inv Hbv; auto.
+    - right. intro. apply H. inv H0. auto.
+    - 
+      assert (Hn := Decidable_name_in_fundefs f4).
+      inv Hn. specialize (Dec x). inv Dec.
+      left; auto. 
+      right. intro. apply H. inv H1. exfalso; auto. auto.
+    -
+      assert (Hf5 := Decidable_name_in_fundefs_ctx f5). inv Hf5. specialize (Dec x). inv Dec.
+      left.
+      constructor. auto.
+      right. intro; apply H. inv H1.
+      exfalso; auto. auto.
+    -  destruct (in_dec var_dec x l); auto.
+       right; intro. apply H. inv H0. exfalso; auto. auto.
+    - right.
+      intro; apply H. inv H0. auto.
+  Qed.
+
+  Lemma bound_stem_ctx_dec:
+    (forall c, Decidable (bound_stem_ctx c)).
+  Proof.
+    intro. apply bound_stem_ctx_dec_mut.
+  Qed.
+
+
+  Lemma bound_stem_fundefs_ctx_dec:
+    (forall c, Decidable (bound_stem_fundefs_ctx c)).
+  Proof.
+    intro. apply bound_stem_ctx_dec_mut.
+  Qed.
+
+  
+    (** The set of bound variables of a composed context is equal to the union of the sets of bound variables of its constituents *)
+  Theorem bound_stem_comp_ctx_mut:
+    forall c',
+      (forall c,
+         Same_set _ (Union _ (bound_stem_ctx c) (bound_stem_ctx c')) (bound_stem_ctx (comp_ctx_f c c'))) /\
+      (forall fc,
+         Same_set  _ (Union _ (bound_stem_fundefs_ctx fc) (bound_stem_ctx c')) (bound_stem_fundefs_ctx (comp_f_ctx_f fc c'))).
+  Proof.
+    intro c'; apply exp_fundefs_ctx_mutual_ind; intros; simpl; repeat normalize_bound_stem_ctx'; eauto 25 with Ensembles_DB.
+    -  rewrite <- H.
+       rewrite <- Union_assoc.
+       rewrite Union_commut with (s1 := [set v]).
+       eauto 25 with Ensembles_DB.
+    - rewrite <- H.
+      rewrite <- Union_assoc.
+      rewrite Union_commut with (s1 := [set v]).
+      eauto 25 with Ensembles_DB.
+    -  rewrite <- H.
+       rewrite <- Union_assoc.
+       rewrite Union_commut with (s1 := [set v]).
+       eauto 25 with Ensembles_DB. 
+    -   rewrite <- H.
+        rewrite <- Union_assoc.
+        reflexivity.
+    - assert (Hf5 := name_in_fundefs_ctx_comp c' f5).
+      rewrite Hf5.
+      rewrite <- H.
+      eauto 25 with Ensembles_DB.
+    - rewrite <- H.
+      split;
+        eauto 25 with Ensembles_DB.
+  Qed.
